steel/Zeta.Steel.Verifier.fst
@@ -19,11 +19,491 @@ module AEH = Zeta.Steel.AggregateEpochHashes
 module P = Zeta.Steel.Parser
 module Cast = FStar.Int.Cast
 open Zeta.Steel.EpochHashes
+module Application = Zeta.Steel.Application
+#push-options "--ide_id_info_off"
 let spec_parser_log  = admit()
-let bytes_from (b:bytes)
-               (l:U32.t { U32.v l <= Seq.length b })
-  : bytes
-  = Seq.slice b (U32.v l) (Seq.length b)
+
+let compat_with_any_anchor_of_le (l:TLM.log)
+                                 (le:log_entry { not (VerifyEpoch? le) })
+  : Lemma (l `TLM.log_grows` (Seq.snoc l le) /\
+           (Seq.snoc l le) `TLM.compat_with_any_anchor_of` l)
+          [SMTPat (Seq.snoc l le)]
+  = admit()
+
+let fail (#p:prop)
+         (#tsm:M.thread_state_model)
+         (#entries:erased _)
+         (#tid:erased _)
+         (t:thread_state_t)
+         (aeh:AEH.aggregate_epoch_hashes) //lock & handle to the aggregate state
+         (#outlen:U32.t)
+         (#out_bytes:erased _)
+         (out:larray U8.t outlen) //out array, to write outputs
+  : STT unit
+    (thread_state_inv t tsm `star`
+     TLM.tid_pts_to aeh.mlogs tid full entries false `star`
+     array_pts_to out out_bytes `star`
+     pure p)
+    (fun _ ->
+      exists_ (thread_state_inv t) `star`
+      exists_ (array_pts_to out) `star`
+      exists_ (fun entries -> TLM.tid_pts_to aeh.mlogs tid full entries false))
+  = intro_exists _ (thread_state_inv t);
+    intro_exists _ (fun entries -> TLM.tid_pts_to aeh.mlogs tid full entries false);
+    intro_exists _ (array_pts_to out);
+    elim_pure _;
+    ()
+
+let intro_nout_bytes //(#o:_)
+                     (tsm tsm':M.thread_state_model)
+                     (out_bytes:erased bytes)
+  : ST unit
+    emp
+    (fun _ -> pure (Application.n_out_bytes tsm tsm' 0ul out_bytes out_bytes))
+    (requires Application.delta_out_bytes tsm tsm' == Seq.empty)
+    (ensures fun _ -> True)
+  = admit__()
+
+let verify_log_entry_post (tsm:M.thread_state_model)
+                          (t:thread_state_t)
+                          (#outlen:U32.t)
+                          (out_bytes0:bytes)
+                          (out:larray U8.t outlen) //out array, to write outputs
+                          (aeh:AEH.aggregate_epoch_hashes) //lock & handle to the aggregate state
+                          (le:LogEntry.log_entry)
+                          ([@@@smt_fallback] res:option U32.t)
+  : vprop
+  = match res with
+    | None ->
+         //if it fails, you still get back ownership on the various
+         //resources, e.g., to free them
+         //but not much else
+         exists_ (thread_state_inv t) `star`
+         exists_ (array_pts_to out) `star`
+         exists_ (fun entries -> TLM.tid_pts_to aeh.mlogs tsm.thread_id full entries false)
+
+    | Some n_out ->
+         //it succeeded
+         let tsm' = M.verify_step_model tsm le in
+         exists_ (fun (out_bytes1:Seq.seq U8.t) ->
+           thread_state_inv t tsm' `star` //tsm' is the new state of the thread
+           array_pts_to out out_bytes1 `star`  //the out array contains out_bytes
+           TLM.tid_pts_to aeh.mlogs tsm.thread_id full tsm'.processed_entries false `star` //my contributions are updated
+           pure (Application.n_out_bytes tsm tsm' n_out out_bytes0 out_bytes1))
+
+let success (#o:_)
+            (#tsm:M.thread_state_model)
+            (t:thread_state_t)
+            (aeh:AEH.aggregate_epoch_hashes) //lock & handle to the aggregate state
+            (#outlen:U32.t)
+            (#out_bytes0 #out_bytes1:erased _)
+            (out:larray U8.t outlen) //out array, to write outputs
+            (le:log_entry)
+            (n_out:U32.t)
+  : STGhostT unit o
+    (thread_state_inv t (M.verify_step_model tsm le) `star`
+     TLM.tid_pts_to aeh.mlogs tsm.thread_id full (M.verify_step_model tsm le).processed_entries false `star`
+     array_pts_to out out_bytes1 `star`
+     pure (Application.n_out_bytes tsm (M.verify_step_model tsm le) n_out out_bytes0 out_bytes1))
+    (fun _ ->
+      verify_log_entry_post tsm t out_bytes0 out aeh le (Some n_out))
+       // let tsm' = M.verify_step_model tsm le in
+       // exists_ (fun (out_bytes1:Seq.seq U8.t) ->
+       //   thread_state_inv t tsm' `star` //tsm' is the new state of the thread
+       //   array_pts_to out out_bytes1 `star`  //the out array contains out_bytes
+       //   TLM.tid_pts_to aeh.mlogs tsm.thread_id full tsm'.processed_entries false `star` //my contributions are updated
+       //   pure (Application.n_out_bytes tsm tsm' n_out out_bytes0 out_bytes1)))
+  = let tsm' = M.verify_step_model tsm le in
+    intro_exists_erased out_bytes1
+       (fun (out_bytes1:Seq.seq U8.t) ->
+         thread_state_inv t tsm' `star` //tsm' is the new state of the thread
+         array_pts_to out out_bytes1 `star`  //the out array contains out_bytes
+         TLM.tid_pts_to aeh.mlogs tsm.thread_id full tsm'.processed_entries false `star` //my contributions are updated
+         pure (Application.n_out_bytes tsm tsm' n_out out_bytes0 out_bytes1))
+
+#push-options "--query_stats --fuel 2 --ifuel 2 --z3rlimit_factor 3"
+let snoc_entries (tsm:M.thread_state_model {not tsm.failed})
+                 (le:log_entry)
+  : Lemma (ensures (M.verify_step_model tsm le).processed_entries ==
+                    Seq.snoc tsm.processed_entries le)
+  = match le with
+    | RunApp pl ->
+      let rec write_slots_processed_entries_framing
+              (tsm:M.thread_state_model)
+              (slots:Seq.seq slot_id { forall (s:U16.t). {:pattern Seq.contains slots s}
+                                                Seq.contains slots s ==>
+                                                M.has_slot tsm s /\
+                                                ApplicationKey? (M.key_of_slot tsm s)
+                               })
+              (values:Seq.seq (Zeta.App.app_value_nullable aprm.adm) {
+                                                     Seq.length slots == Seq.length values
+                        })
+      : Lemma (ensures (
+                       let tsm' = M.write_slots tsm slots values in
+                       tsm'.processed_entries == tsm.processed_entries))
+              (decreases (Seq.length slots))
+      = if Seq.length slots = 0 then ()
+        else (
+          let hd_slot = Seq.head slots in
+          let tl = Seq.tail slots in
+          assert (slots `Seq.equal` Seq.cons hd_slot tl);
+          Classical.forall_intro (Seq.contains_cons hd_slot tl);
+          let hd_value =
+            match Seq.head values with
+            | Zeta.App.Null -> DValue None
+            | Zeta.App.DValue d -> DValue (Some d)
+          in
+          let tsm = M.update_value tsm hd_slot hd_value in
+          write_slots_processed_entries_framing tsm tl (Seq.tail values)
+        )
+      in
+      let tsm' = M.runapp tsm pl in
+      if not (Map.contains aprm.tbl pl.fid)
+      then ()
+      else (
+        match spec_app_parser pl.fid pl.rest.ebytes with
+        | None -> ()
+        | Some ((arg, slots), len) ->
+          if len <> U32.v pl.rest.len
+          then ()
+          else (
+            if not (Zeta.SeqAux.distinct_elems_comp slots)
+            then ()
+            else (
+              let fsig = Map.sel aprm.tbl pl.fid in
+              match M.read_slots tsm slots with
+              | None -> ()
+              | Some recs ->
+                if not (M.check_distinct_keys recs)
+                then ()
+                else (
+                  let res = fsig.f arg recs in
+                  match res with
+                  | ( Zeta.App.Fn_failure, _, _) -> ()
+                  | ( _, res, out_vals) ->
+                    let tsm'' = {tsm with app_results = Seq.snoc tsm.app_results (| pl.fid, arg, recs, res |) } in
+                    assert (tsm' == M.write_slots tsm'' slots out_vals);
+                    assert (tsm''.processed_entries == tsm.processed_entries);
+                    write_slots_processed_entries_framing tsm'' slots out_vals;
+                    assert (tsm'.processed_entries == tsm''.processed_entries)
+                )
+            )
+          )
+        )
+    | _ ->
+      ()
+#pop-options
+
+
+val verify_entry_cases (#tsm:M.thread_state_model)
+                       (t:thread_state_t) //handle to the thread state
+                       (#outlen:U32.t)
+                       (#out_bytes0:erased bytes)
+                       (out:larray U8.t outlen) //out array, to write outputs
+                       (aeh:AEH.aggregate_epoch_hashes) //lock & handle to the aggregate state
+                       (le:LogEntry.log_entry)
+                       (b:bool)
+  : ST (option U32.t)
+    (thread_state_inv t (update_if b tsm (M.verify_step_model tsm le)) `star`
+     TLM.tid_pts_to aeh.mlogs tsm.thread_id full tsm.processed_entries false `star`
+     array_pts_to out out_bytes0)
+    (fun res -> verify_log_entry_post tsm t out_bytes0 out aeh le res)
+    (requires
+      not (VerifyEpoch? le) /\ not (RunApp? le) /\
+      not tsm.failed)
+    (ensures fun _ -> True)
+//fusing val and let leads to errors
+let verify_entry_cases (#tsm:M.thread_state_model)
+                       (t:thread_state_t) //handle to the thread state
+                       (#outlen:U32.t)
+                       (#out_bytes0:erased bytes)
+                       (out:larray U8.t outlen) //out array, to write outputs
+                       (aeh:AEH.aggregate_epoch_hashes) //lock & handle to the aggregate state
+                       (le:LogEntry.log_entry)
+                       (b:bool)
+  = snoc_entries tsm le;
+    compat_with_any_anchor_of_le tsm.processed_entries le;
+    TLM.update_tid_log aeh.mlogs tsm.thread_id tsm.processed_entries (M.verify_step_model tsm le).processed_entries;
+    intro_nout_bytes tsm (M.verify_step_model tsm le) out_bytes0;
+    if b
+    then (
+      rewrite (thread_state_inv t _)
+              (thread_state_inv t (M.verify_step_model tsm le));
+      success t aeh out le 0ul;
+      return (Some 0ul)
+    )
+    else (
+      rewrite (thread_state_inv t _)
+              (thread_state_inv t tsm);
+      fail t aeh out;
+      return None
+    )
+
+val verify_log_entry (#tsm:M.thread_state_model)
+                     (t:thread_state_t) //handle to the thread state
+                     (#outlen:U32.t)
+                     (#outbytes0:erased bytes)
+                     (out:larray U8.t outlen) //out array, to write outputs
+                     (aeh:AEH.aggregate_epoch_hashes) //lock & handle to the aggregate state
+                     (le:LogEntry.log_entry)
+  : ST (option U32.t)
+    (//precondition
+      thread_state_inv t tsm `star` //thread state is initially tsm
+      array_pts_to out outbytes0 `star` //we have permission to out, don't care what it contains
+      TLM.tid_pts_to aeh.mlogs tsm.thread_id full tsm.processed_entries false //and the global state contains this thread's entries
+    )
+    (fun res -> //postcondition
+      verify_log_entry_post tsm t outbytes0 out aeh le res)
+    (requires not tsm.failed /\
+              not (RunApp? le))
+    (ensures fun _ -> True)
+
+#push-options "--query_stats --fuel 0 --ifuel 1 --z3rlimit_factor 3"
+
+let verify_log_entry (#tsm:M.thread_state_model)
+                     (t:thread_state_t) //handle to the thread state
+                     (#outlen:U32.t)
+                     (#out_bytes:erased bytes)
+                     (out:larray U8.t outlen) //out array, to write outputs
+                     (aeh:AEH.aggregate_epoch_hashes) //lock & handle to the aggregate state
+                     (le:LogEntry.log_entry)
+   = snoc_entries tsm le;
+     match le with
+     | VerifyEpoch ->
+       let b = VerifierSteps.verify_epoch t aeh in
+       intro_nout_bytes tsm (M.verify_step_model tsm le) out_bytes;
+       if b
+       then (
+         rewrite (thread_state_inv t _)
+                 (thread_state_inv t (M.verify_step_model tsm le));
+         success t aeh out le 0ul;
+         return (Some 0ul)
+       )
+       else (
+         rewrite (thread_state_inv t _)
+                 (thread_state_inv t tsm);
+         fail t aeh out;
+         return None
+       )
+
+     | _ ->
+       // compat_with_any_anchor_of_le tsm.processed_entries le;
+       // TLM.update_tid_log aeh.mlogs tsm.thread_id tsm.processed_entries (M.verify_step_model tsm le).processed_entries;
+       // intro_nout_bytes tsm (M.verify_step_model tsm le) out_bytes;
+       match le with
+       | AddM s s' r ->
+         let b = VerifierSteps.vaddm t s s' r in
+         verify_entry_cases t out aeh le b
+
+       | AddB s ts tid r ->
+         let b = VerifierSteps.vaddb t s ts tid r in
+         verify_entry_cases t out aeh le b
+
+       | EvictM pl ->
+         VerifierSteps.vevictm t pl.s pl.s';
+         verify_entry_cases t out aeh le true
+
+       | EvictB pl ->
+         let b = VerifierSteps.vevictb t pl.s pl.t in
+         verify_entry_cases t out aeh le b
+
+       | EvictBM pl ->
+         let b = VerifierSteps.vevictbm t pl.s pl.s' pl.t in
+         verify_entry_cases t out aeh le b
+
+       | NextEpoch ->
+         let b = VerifierSteps.nextepoch t in
+         verify_entry_cases t out aeh le true
+
+type verify_step_result =
+  | Parsing_failure: verify_step_result
+  | App_failure: verify_step_result
+  | Verify_log_entry_failure: verify_step_result
+  | Verify_log_entry_success: read:U32.t -> wrote:U32.t -> verify_step_result
+
+let verify_step_post (tsm:M.thread_state_model)
+                     (t:thread_state_t) //handle to the thread state
+                     (log_perm:perm)
+                     (log_bytes:bytes)
+                     (#len:U32.t)
+                     (log_pos:U32.t{U32.v log_pos < Seq.length log_bytes})
+                     (log:larray U8.t len) //concrete log
+                     (#outlen:U32.t)
+                     (out_bytes:bytes)
+                     (out:larray U8.t outlen) //out array, to write outputs
+                     (aeh:AEH.aggregate_epoch_hashes) //lock & handle to the aggregate state
+                     ([@@@smt_fallback] res:verify_step_result)
+ : vprop
+ = match res with
+   | Parsing_failure ->
+      pure (LogEntry.spec_parser_log_entry (Parser.bytes_from log_bytes log_pos) == None) `star`
+      thread_state_inv t tsm `star`
+      TLM.tid_pts_to aeh.mlogs tsm.thread_id full tsm.processed_entries false `star`
+      array_pts_to out out_bytes
+
+   | App_failure ->
+      thread_state_inv t tsm `star`
+      TLM.tid_pts_to aeh.mlogs tsm.thread_id full tsm.processed_entries false `star`
+      array_pts_to out out_bytes
+
+   | Verify_log_entry_failure ->
+      (match (LogEntry.spec_parser_log_entry (Parser.bytes_from log_bytes log_pos)) with
+       | None -> pure False
+       | Some (le, _) -> verify_log_entry_post tsm t out_bytes out aeh le None)
+
+   | Verify_log_entry_success read wrote ->
+      (match (LogEntry.spec_parser_log_entry (Parser.bytes_from log_bytes log_pos)) with
+       | None -> pure False
+       | Some _ ->
+         pure (snd (LogEntry.spec_parse_log_entry log_bytes log_pos) == U32.v read) `star`
+         verify_log_entry_post tsm t out_bytes out aeh
+           (fst (LogEntry.spec_parse_log_entry log_bytes log_pos))
+           (Some wrote))
+
+let intro_verify_step_post_parsing_failure
+                     (#o:_)
+                     (#tsm:M.thread_state_model)
+                     (t:thread_state_t) //handle to the thread state
+                     (#log_perm:perm)
+                     (#log_bytes:erased bytes)
+                     (#len:U32.t)
+                     (log_pos:U32.t{U32.v log_pos < Seq.length log_bytes})
+                     (log:larray U8.t len) //concrete log
+                     (#outlen:U32.t)
+                     (out_bytes:bytes)
+                     (out:larray U8.t outlen) //out array, to write outputs
+                     (aeh:AEH.aggregate_epoch_hashes) //lock & handle to the aggregate state
+  : STGhost unit o
+    (thread_state_inv t tsm `star`
+     TLM.tid_pts_to aeh.mlogs tsm.thread_id full tsm.processed_entries false `star`
+     array_pts_to out out_bytes)
+    (fun _ ->
+      verify_step_post tsm t log_perm log_bytes log_pos log out_bytes out aeh Parsing_failure)
+    (requires
+      LogEntry.spec_parser_log_entry (Parser.bytes_from log_bytes log_pos) == None)
+    (ensures fun _ -> True)
+  = intro_pure (LogEntry.spec_parser_log_entry (Parser.bytes_from log_bytes log_pos) == None);
+    rewrite (pure _ `star`
+             thread_state_inv t tsm `star`
+             TLM.tid_pts_to aeh.mlogs tsm.thread_id full tsm.processed_entries false `star`
+             array_pts_to out out_bytes)
+             _
+
+let intro_verify_step_post_app_failure
+                     (#o:_)
+                     (#tsm:M.thread_state_model)
+                     (t:thread_state_t) //handle to the thread state
+                     (#log_perm:perm)
+                     (#log_bytes:erased bytes)
+                     (#len:U32.t)
+                     (log_pos:U32.t{U32.v log_pos < Seq.length log_bytes})
+                     (log:larray U8.t len) //concrete log
+                     (#outlen:U32.t)
+                     (out_bytes:bytes)
+                     (out:larray U8.t outlen) //out array, to write outputs
+                     (aeh:AEH.aggregate_epoch_hashes) //lock & handle to the aggregate state
+  : STGhostT unit o
+    (thread_state_inv t tsm `star`
+     TLM.tid_pts_to aeh.mlogs tsm.thread_id full tsm.processed_entries false `star`
+     array_pts_to out out_bytes)
+    (fun _ ->
+      verify_step_post tsm t log_perm log_bytes log_pos log out_bytes out aeh App_failure)
+  = rewrite (thread_state_inv t tsm `star`
+             TLM.tid_pts_to aeh.mlogs tsm.thread_id full tsm.processed_entries false `star`
+             array_pts_to out out_bytes)
+             _
+
+let intro_verify_step_post_verify_failure
+                     (#o:_)
+                     (#tsm:M.thread_state_model)
+                     (t:thread_state_t) //handle to the thread state
+                     (#log_perm:perm)
+                     (#log_bytes:erased bytes)
+                     (#len:U32.t)
+                     (log_pos:U32.t{U32.v log_pos < Seq.length log_bytes})
+                     (log:larray U8.t len) //concrete log
+                     (#outlen:U32.t)
+                     (out_bytes:bytes)
+                     (out:larray U8.t outlen) //out array, to write outputs
+                     (aeh:AEH.aggregate_epoch_hashes) //lock & handle to the aggregate state
+                     (le: log_entry)
+  : STGhost unit o
+    (verify_log_entry_post tsm t out_bytes out aeh le None)
+    (fun _ ->
+      verify_step_post tsm t log_perm log_bytes log_pos log out_bytes out aeh Verify_log_entry_failure)
+    (requires
+       (match (LogEntry.spec_parser_log_entry (Parser.bytes_from log_bytes log_pos)) with
+       | None -> False
+       | Some (le', n') -> le == le'))
+    (ensures fun _ -> True)
+  = rewrite _ _
+
+let intro_verify_step_post_verify_success
+                     (#o:_)
+                     (#tsm:M.thread_state_model)
+                     (t:thread_state_t) //handle to the thread state
+                     (#log_perm:perm)
+                     (#log_bytes:erased bytes)
+                     (#len:U32.t)
+                     (log_pos:U32.t{U32.v log_pos < Seq.length log_bytes})
+                     (log:larray U8.t len) //concrete log
+                     (#outlen:U32.t)
+                     (out_bytes:bytes)
+                     (out:larray U8.t outlen) //out array, to write outputs
+                     (aeh:AEH.aggregate_epoch_hashes) //lock & handle to the aggregate state
+                     (le: log_entry)
+                     (n_read:U32.t)
+                     (n_written:U32.t)
+  : STGhost unit o
+    (verify_log_entry_post tsm t out_bytes out aeh le (Some n_written))
+    (fun _ ->
+      verify_step_post tsm t log_perm log_bytes log_pos log out_bytes out aeh (Verify_log_entry_success n_read n_written))
+    (requires
+       LogEntry.can_parse_log_entry log_bytes log_pos /\
+       LogEntry.spec_parse_log_entry log_bytes log_pos == (le, U32.v n_read))
+    (ensures fun _ -> True)
+  = intro_pure (snd (LogEntry.spec_parse_log_entry log_bytes log_pos) == U32.v n_read);
+    rewrite (pure _ `star`
+             verify_log_entry_post tsm t out_bytes out aeh le (Some n_written))
+             _
+
+let intro_verify_step_post_runapp_success
+                     (#o:_)
+                     (#tsm:M.thread_state_model)
+                     (t:thread_state_t) //handle to the thread state
+                     (#log_perm:perm)
+                     (#log_bytes:erased bytes)
+                     (#len:U32.t)
+                     (log_pos:U32.t{U32.v log_pos < Seq.length log_bytes})
+                     (log:larray U8.t len) //concrete log
+                     (#outlen:U32.t)
+                     (out_bytes:bytes)
+                     (out:larray U8.t outlen) //out array, to write outputs
+                     (aeh:AEH.aggregate_epoch_hashes) //lock & handle to the aggregate state
+                     (le: log_entry)
+                     (n_read:U32.t)
+                     (n_written:U32.t)
+                     (res:Application.verify_runapp_result)
+  : STGhost unit o
+    (Application.verify_runapp_entry_post tsm t #len log_pos log_bytes out_bytes out res `star`
+     TLM.tid_pts_to aeh.mlogs tsm.thread_id full tsm.processed_entries false)
+    (fun _ ->
+      verify_step_post tsm t log_perm log_bytes log_pos log out_bytes out aeh (Verify_log_entry_success n_read n_written))
+    (requires res == Application.Run_app_success n_read n_written /\ not tsm.failed)
+    (ensures fun _ -> True)
+  = rewrite (Application.verify_runapp_entry_post tsm t #len log_pos log_bytes out_bytes out res)
+            (Application.verify_runapp_entry_post tsm t #len log_pos log_bytes out_bytes out (Application.Run_app_success n_read n_written));
+    let pl = elim_exists () in
+    let out_bytes' = elim_exists () in
+    elim_pure _;
+    assert_ (thread_state_inv t (M.verify_step_model tsm (RunApp pl)));
+    assert_ (array_pts_to out out_bytes');
+    snoc_entries tsm (RunApp pl);
+    compat_with_any_anchor_of_le tsm.processed_entries (RunApp pl);
+    TLM.update_tid_log aeh.mlogs tsm.thread_id tsm.processed_entries (M.verify_step_model tsm (RunApp pl)).processed_entries;
+    intro_pure (Application.n_out_bytes tsm (M.verify_step_model tsm (RunApp pl)) n_written  out_bytes out_bytes');
+    success t aeh out (RunApp pl) n_written;
+    intro_verify_step_post_verify_success #_ #tsm t #log_perm #log_bytes #len log_pos log #outlen out_bytes out aeh (RunApp pl) n_read n_written
 
 val verify_step (#tsm:M.thread_state_model)
                 (t:thread_state_t) //handle to the thread state
@@ -33,44 +513,23 @@ val verify_step (#tsm:M.thread_state_model)
                 (log_pos:U32.t{U32.v log_pos < Seq.length log_bytes})
                 (log:larray U8.t len) //concrete log
                 (#outlen:U32.t)
+                (#out_bytes:erased bytes)
+                (out_pos:U32.t{U32.v out_pos < Seq.length out_bytes})
                 (out:larray U8.t outlen) //out array, to write outputs
                 (aeh:AEH.aggregate_epoch_hashes) //lock & handle to the aggregate state
-  : STT (option (U32.t & U32.t))
+  : ST verify_step_result
     (//precondition
       A.pts_to log log_perm log_bytes `star` //the log contains log_bytes
       thread_state_inv t tsm `star` //thread state is initially tsm
-      exists_ (array_pts_to out) `star` //we have permission to out, don't care what it contains
+      array_pts_to out out_bytes `star` //we have permission to out, don't care what it contains
       TLM.tid_pts_to aeh.mlogs tsm.thread_id full tsm.processed_entries false //and the global state contains this thread's entries
     )
     (fun res -> //postcondition
       A.pts_to log log_perm log_bytes `star` //log contents didn't change
-      (match res with
-       | None ->
-         //if it fails, you still get back ownership on the various
-         //resources, e.g., to free them
-         //but not much else
-         exists_ (thread_state_inv t) `star`
-         exists_ (array_pts_to out)
-      | Some (n_read, n_out) ->
-         //it succeeded
-         exists_ (fun (tsm':M.thread_state_model) ->
-         exists_ (fun (out_bytes:Seq.seq U8.t) ->
-           thread_state_inv t tsm' `star` //tsm' is the new state of the thread
-           array_pts_to out out_bytes `star`  //the out array contains out_bytes
-           TLM.tid_pts_to aeh.mlogs tsm.thread_id full tsm'.processed_entries false `star` //my contributions are updated
-           pure (
-             match LogEntry.spec_parser_log_entry (bytes_from log_bytes log_pos) with
-             | None -> False //log parsing did not fail
-             | Some (log_entry, n_read') -> //parsing produces log_entries
-               U32.v n_read == n_read' /\
-               //tsm' what you get by running the spec verifier from tsm on log_entries
-               tsm' == M.verify_step_model tsm log_entry /\
-               //the out_bytes contain any new app results in tsm'
-               out_bytes == M.bytes_of_app_results (M.delta_app_results tsm tsm') /\
-               //and n_out is the number of bytes that were written
-               U32.v n_out == Seq.length out_bytes
-           )
-           ))))
+      verify_step_post tsm t log_perm log_bytes log_pos log out_bytes out aeh res)
+    (requires not tsm.failed)
+    (ensures fun _ -> True)
+
 let verify_step (#tsm:M.thread_state_model)
                 (t:thread_state_t) //handle to the thread state
                 (#log_perm:perm)
@@ -78,7 +537,53 @@ let verify_step (#tsm:M.thread_state_model)
                 (#len:U32.t)
                 (log_pos:U32.t{U32.v log_pos < Seq.length log_bytes})
                 (log:larray U8.t len) //concrete log
-                (#outlen:U32.t)
-                (out:larray U8.t outlen) //out array, to write outputs
+                (#out_len:U32.t)
+                (#out_bytes:erased bytes)
+                (out_pos:U32.t{U32.v out_pos < Seq.length out_bytes})
+                (out:larray U8.t out_len) //out array, to write outputs
                 (aeh:AEH.aggregate_epoch_hashes) //lock & handle to the aggregate state
-    = admit__()
+    = A.pts_to_length log _;
+      let res = LogEntry.parser_log_entry len log_pos U32.(len -^ log_pos) log in
+      match res with
+      | None ->
+        intro_verify_step_post_parsing_failure t log_pos log out_bytes out aeh;
+        return Parsing_failure
+
+      | Some (le, read) ->
+        match le with
+        | RunApp _ ->
+          let app_res =
+            Application.run_app_function
+              len log_pos log
+              out_len 0ul out
+              t
+          in
+          begin
+          match app_res with
+          | Application.Run_app_parsing_failure
+          | Application.Run_app_verify_failure ->
+            rewrite (Application.verify_runapp_entry_post _ _ _ _ _ _ _)
+                    (thread_state_inv t tsm `star`
+                     array_pts_to out out_bytes);
+            intro_verify_step_post_app_failure t log_pos log out_bytes out aeh;
+            return App_failure
+
+          | Application.Run_app_success read written ->
+//            assert_ (Application.verify_runapp_entry_post tsm t log_pos log_bytes out_bytes out app_res);
+            let _ = intro_verify_step_post_runapp_success #_ #tsm t #log_perm #log_bytes log_pos log out_bytes out aeh le read written app_res in
+            return (Verify_log_entry_success read written)
+          end
+
+        | _ ->
+          let b = verify_log_entry t out aeh le in
+          match b with
+          | None ->
+            rewrite (verify_log_entry_post tsm t out_bytes out aeh le b)
+                    (verify_step_post tsm t log_perm log_bytes log_pos log out_bytes out aeh Verify_log_entry_failure);
+            return Verify_log_entry_failure
+
+          | Some written ->
+            rewrite (verify_log_entry_post tsm t out_bytes out aeh le b)
+                    (verify_log_entry_post tsm t out_bytes out aeh le (Some written));
+            intro_verify_step_post_verify_success t #log_perm log_pos log out_bytes out aeh le read written;
+            return (Verify_log_entry_success read written)
