steel/Zeta.Steel.LogEntry.Spec.fsti
@@ -1,5 +1,18 @@
 module Zeta.Steel.LogEntry.Spec
 include Zeta.Steel.LogEntry.Types
 open Zeta.Steel.Parser
-
+module U32 = FStar.UInt32
 val spec_parser_log_entry : spec_parser log_entry
+
+let can_parse_log_entry (log_bytes:bytes)
+                        (log_pos:U32.t{  U32.v log_pos < Seq.length log_bytes })
+  : prop
+  = Some? (spec_parser_log_entry (Zeta.Steel.Parser.bytes_from log_bytes log_pos)) == true
+
+let spec_parse_log_entry (log_bytes:bytes)
+                         (log_pos:U32.t{
+                            U32.v log_pos < Seq.length log_bytes /\
+                            can_parse_log_entry log_bytes log_pos
+                          })
+  : GTot (log_entry & nat)
+  = parse_result log_bytes log_pos spec_parser_log_entry
