steel/Zeta.Steel.VerifierSteps.fsti
@@ -7,6 +7,8 @@ open Zeta.Steel.FormatsManual
 open Zeta.Steel.Util
 module M = Zeta.Steel.ThreadStateModel
 module T = Zeta.Steel.FormatsManual
+module AEH = Zeta.Steel.AggregateEpochHashes
+module TLM = Zeta.Steel.ThreadLogMap
 #push-options "--ide_id_info_off"
 
 val create (tid:tid)
@@ -19,10 +21,10 @@ val vaddm (#tsm:M.thread_state_model)
           (s s':slot_id)
           (r:T.record)
   : STT bool
-    (thread_state_inv_core t tsm)
+    (thread_state_inv t tsm)
     (fun b ->
-      thread_state_inv_core t
-           (update_if b tsm (M.vaddm tsm s s' r)))
+      thread_state_inv t
+           (update_if b tsm (M.verify_step_model tsm (AddM s s' r))))
 
 val vaddb (#tsm:M.thread_state_model)
           (t:thread_state_t)
@@ -31,50 +33,39 @@ val vaddb (#tsm:M.thread_state_model)
           (thread_id:T.thread_id)
           (r:T.record)
   : STT bool
-       (thread_state_inv_core t tsm)
+       (thread_state_inv t tsm)
        (fun b ->
-         thread_state_inv_core t
-               (update_if b tsm (M.vaddb tsm s ts thread_id r)))
+         thread_state_inv t
+               (update_if b tsm (M.verify_step_model tsm (AddB s ts thread_id r))))
 
 val vevictm (#tsm:M.thread_state_model)
             (t:thread_state_t)
             (s s':slot_id)
   : STT unit
-    (thread_state_inv_core t tsm)
-    (fun _ -> thread_state_inv_core t (M.vevictm tsm s s'))
+    (thread_state_inv t tsm)
+    (fun _ -> thread_state_inv t (M.verify_step_model tsm (EvictM ({s; s'}))))
 
 val vevictb (#tsm:M.thread_state_model)
             (t:thread_state_t)
             (s:slot_id)
             (ts:timestamp)
-  : ST bool
-    (thread_state_inv_core t tsm)
-    (fun b -> thread_state_inv_core t (update_if b tsm (M.vevictb tsm s ts)))
-    (requires VerifierTypes.thread_id t == tsm.thread_id)
-    (ensures fun _ -> True)
+  : STT bool
+    (thread_state_inv t tsm)
+    (fun b -> thread_state_inv t (update_if b tsm (M.verify_step_model tsm (EvictB ({s; t=ts})))))
 
 val vevictbm (#tsm:M.thread_state_model)
              (t:thread_state_t)
              (s s':slot_id)
              (ts:timestamp)
-  : ST bool
-    (thread_state_inv_core t tsm)
-    (fun b -> thread_state_inv_core t (update_if b tsm (M.vevictbm tsm s s' ts)))
-    (VerifierTypes.thread_id t == tsm.thread_id)
-    (fun _ -> True)
+  : STT bool
+    (thread_state_inv t tsm)
+    (fun b -> thread_state_inv t (update_if b tsm (M.verify_step_model tsm (EvictBM ({s; s'; t=ts})))))
 
 val nextepoch (#tsm:M.thread_state_model)
               (t:thread_state_t)
   : STT unit
-    (thread_state_inv_core t tsm)
-    (fun _ -> thread_state_inv_core t (M.nextepoch tsm))
-
-module AEH = Zeta.Steel.AggregateEpochHashes
-module TLM = Zeta.Steel.ThreadLogMap
-let spec_verify_epoch (tsm:M.thread_state_model)
-  = let tsm = M.verifyepoch tsm in
-    if tsm.failed then tsm
-    else { tsm with M.processed_entries = Seq.snoc tsm.processed_entries (VerifyEpoch)}
+    (thread_state_inv t tsm)
+    (fun _ -> thread_state_inv t (M.verify_step_model tsm NextEpoch))
 
 val verify_epoch (#tsm:M.thread_state_model)
                  (t:thread_state_t)
@@ -83,9 +74,9 @@ val verify_epoch (#tsm:M.thread_state_model)
     (thread_state_inv t tsm `star`
      TLM.tid_pts_to aeh.mlogs tsm.thread_id full tsm.processed_entries false)
     (fun b ->
-      thread_state_inv t (update_if b tsm (spec_verify_epoch tsm)) `star`
+      thread_state_inv t (update_if b tsm (M.verify_step_model tsm VerifyEpoch)) `star`
       TLM.tid_pts_to aeh.mlogs tsm.thread_id full (update_if b tsm.processed_entries
-                                                         (spec_verify_epoch tsm).processed_entries)
+                                                         (M.verify_step_model tsm VerifyEpoch).processed_entries)
                                             false)
     (requires not tsm.failed)
     (ensures fun _ -> True)
